% !TeX encoding = UTF-8
% !TeX program = XeLaTeX
% !TeX spellcheck = LaTeX

\documentclass[a4paper]{article}

\usepackage{amsmath,amsfonts,amssymb}
\usepackage{mathrsfs}
\usepackage{bm}
\usepackage{extarrows}
\usepackage{geometry}
\usepackage{ntheorem}
\usepackage{hyperref}
\usepackage[ruled]{algorithm2e}
\usepackage{caption,subcaption}

\geometry{left=2cm,right=2cm,top=2cm,bottom=2cm}

\def\UrlBreaks{\do\A\do\B\do\C\do\D\do\E\do\F\do\G\do\H\do\I\do\J\do\K\do\L\do\M\do\N\do\O\do\P\do\Q\do\R\do\S\do\T\do\U\do\V\do\W\do\X\do\Y\do\Z\do\[\do\\\do\]\do\^\do\_\do\`\do\a\do\b\do\c\do\d\do\e\do\f\do\g\do\h\do\i\do\j\do\k\do\l\do\m\do\n\do\o\do\p\do\q\do\r\do\s\do\t\do\u\do\v\do\w\do\x\do\y\do\z\do\0\do\1\do\2\do\3\do\4\do\5\do\6\do\7\do\8\do\9\do\.\do\@\do\\\do\/\do\!\do\_\do\|\do\;\do\>\do\]\do\)\do\,\do\?\do\'\do+\do\=\do\#}

\newtheorem{theorem}{Theorem}
\newtheorem{lemma}{Lemma}
\newtheorem{proposition}{Proposition}
\newtheorem{corollary}{Corollary}
\newtheorem{claim}{Claim}
\newtheorem{conjecture}{conjecture}
\newtheorem{definition}{Definition}
\newtheorem{construction}{Construction}
\newtheorem*{proof}{Proof}
\newtheorem*{answer}{Answer}
\newtheorem*{example}{Example}
\newtheorem*{counterexample}{Counterexample}

\newenvironment{exercise}[1]{
	\par
	\noindent\textbf{Exercise #1.}\quad
}{
	\par
	\bigskip
}
\newenvironment{problem}[1]{
	\par
	\noindent\textbf{Problem #1.}\quad
}{
	\par
	\bigskip
}

\DeclareMathAccent{\widehat}{\mathord}{largesymbols}{"62}
\DeclareMathOperator*{\argmax}{\arg\,\max}
\DeclareMathOperator*{\argmin}{\arg\,\min}
\DeclareMathOperator{\E}{\mathbb E}
\DeclareMathOperator{\Var}{\mathrm{Var}}
\DeclareMathOperator{\tr}{\mathrm{tr}}
\newcommand{\abs}[1]{\left| #1 \right|}
\newcommand{\vabs}[1]{\left\| #1 \right\|}
\newcommand{\abra}[1]{\left\langle #1 \right\rangle}
\newcommand{\pbra}[1]{\left( #1 \right)}
\newcommand{\cbra}[1]{\left\{ #1 \right\}}
\newcommand{\sbra}[1]{\left[ #1 \right]}
\newcommand{\floorbra}[1]{\left\lfloor #1 \right\rfloor}
\newcommand{\ceilbra}[1]{\left\lceil #1 \right\rceil}
\newcommand{\bin}{\{0,1\}}
\newcommand{\ZPP}{\mathtt{ZPP}}
\newcommand{\RP}{\mathtt{RP}}
\newcommand{\coRP}{\mathtt{co}\text{-}\mathtt{RP}}
\newcommand{\per}{\text{per}}
\newcommand{\sgn}{\text{sgn}}
\newcommand{\Fbb}{\mathbb{F}}
\newcommand{\Nbb}{\mathbb{N}}
\newcommand{\Rbb}{\mathbb{R}}
\newcommand{\Zbb}{\mathbb{Z}}
\newcommand{\Acal}{\mathcal{A}}
\newcommand{\Bcal}{\mathcal{B}}
\newcommand{\Ccal}{\mathcal{C}}
\newcommand{\Fcal}{\mathcal{F}}
\newcommand{\Gcal}{\mathcal{G}}

\bibliographystyle{plainnat}

\title{Exercise Set --- Chapter $9$}
\date{}

\begin{document}

\maketitle

\begin{exercise}{1}
    \textbf{Remark: This is not the complete solution.}

    Let $\pi_1,\pi_2,\pi_3$ be three independent random permutations in $S_n$.
    Construct a bipartite graph $G=(V_1,V_2,E)$, where $V_1=V_2=[n]$ and 
    $$
    E=\cbra{(i,\pi_1(n)),(i,\pi_2(n)),(i,\pi_3(n))\middle|i\in[n]}.
    $$
    Let $S\subseteq V_1,T\subseteq V_2,|S|+|T|\leq n$ and $0<\delta<1/2$ be a constant to be determined later, then 
    \begin{itemize}
        \item $\max\cbra{|S|,|T|}\geq(\delta+1/2)n$. Then 
            $$
            \frac{|N(S\cup T)|}{|S|+|T|}\geq\frac{N(S)-|T|}{|S|+|T|}\geq\frac{|S|-|T|}{|S|+|T|}\geq2\delta.
            $$
        \item $\max\cbra{|S|,|T|}<\kappa n$. Let $0<\lambda<1/2$ be a constant to be determined later.
            \begin{align*}
                &\Pr\sbra{\exists S,T,\frac{|N(S\cup T)|}{|S|+|T|}<\lambda\middle|\max\cbra{|S|,|T|}<\kappa n}\\
                \leq&2\sum_{|T|\leq|S|<\kappa n}\Pr\sbra{\frac{|N(S\cup T)|}{|S|+|T|}<\lambda}\\
                \leq&2\sum_{|T|\leq|S|<\kappa n}\Pr\sbra{|N(S)|\leq(1+\lambda)|T|+\lambda|S|}\\
                \leq&2\sum_{|S|<\kappa n}\Pr\sbra{|N(S)|\leq(1+2\lambda)|S|}\\
                \leq&2\sum_{i=1}^{\kappa n}\binom ni\binom n{(1+2\lambda)i}\pbra{\frac{(1+2\lambda)i}n}^{3i}.
            \end{align*}
            It can be shown, with $\lambda,\kappa$ sufficiently small, say $\kappa=1/10$, the probability is less than $1$ as $n$ goes to infinity.
        \item $\kappa n\leq\max\cbra{|S|,|T|}<(\delta+1/2)n$. I don't know.
    \end{itemize}
\end{exercise}

\begin{exercise}{2}
    Since $G$ is an $(n,d,\lambda)$-graph, for any $B\subseteq V$ of size $bn$, we have
    $$
    \sum_{v\in V}\abs{|N_B(v)|-bd}^2\leq\lambda^2b(1-b)n.
    $$
    Let $B_c$ be the set of vertices with color $c$,
    then
    \begin{align*}
        \#\cbra{v\middle|N(v)\text{ has $<k$ colors}}
        \leq\sum_{c=1}^k\#\cbra{v\middle|N_{B_c}(v)=\emptyset}
        \leq\sum_{c=1}^k\frac{\lambda^2\frac1k\pbra{1-\frac1k}n}{\frac{d^2}{k^2}}<n.
    \end{align*}
\end{exercise}

\begin{exercise}{3}
    For any fixed $Y,|Y|=5a$.
    Let $X\subseteq V,|X|\leq a$ be any largest subset such that $|N_Y(X)|<2|X|$.
    Then consider any $Z\subset V,Z\cap\pbra{X\cup Y}=\emptyset,|Z|\leq a$.
    \begin{itemize}
        \item $|Z|>|X|$. By the choice of $X$, we have $|N_Y(Z)|\geq2|Z|$.
        \item $|Z|\leq|X|$. Then $X\neq\emptyset$ and $|Z\cup X|>|X|$. 
            \begin{itemize}
                \item $|Z\cup X|\leq a$.
                    Thus by the choice of $X$,
                    $$
                    |N_Y(Z\cup X)|\geq2|Z\cup X|=2|Z|+2|X|.
                    $$
                    Since 
                    $$
                    |N_Y(Z\cup X)|\leq|N_Y(Z)|+|N_Y(X)|<|N_Y(Z)|+2|X|,
                    $$
                    the claim holds as well.
                \item $|Z\cup X|>a$.
                    By assumption, $N_Y(Z\cup X)\neq\emptyset$ and we can repeatedly remove $N_Y(Z\cup X)$ from $Y$
                    until $|Y|\leq a$. Thus
                    $$
                    |N_Y(Z\cup X)|\geq4a.
                    $$
                    On the other hand, $|Z\cup X|\leq 2a$, thus
                    $$
                    |N_Y(Z\cup X)|\leq|N_Y(Z)|+|N_Y(X)|<|N_Y(Z)|+2x\leq|N_Y(Z)|+2(2a-|Z|)
                    $$
                    and then the claim holds as well.
            \end{itemize}
    \end{itemize}
\end{exercise}

\begin{exercise}{4}
    Observe that
    $$
    M=\frac13\sum_{u\in G}|e(N(u))|.
    $$
    Since $G$ is an $(n,n/2,2\sqrt n)$-graph, we have $|N(u)|=n/2$ and
    $$
    \abs{|e(N(u))|-\frac12\times\frac n2\times\pbra{\frac12}^2\times n}\leq\frac12\times2\sqrt n\times\frac n2.
    $$
    Thus 
    $$
    |e(N(u))-\frac{n^2}{16}|=o(n^2)
    $$
    and then
    $$
    \abs{M-\frac{n^3}{48}}=o(n^3),
    $$
    which is equivalent to the original claim.
\end{exercise}

\begin{exercise}{8}
    Here we restate the theorem for convenience.
    \begin{theorem}
        Assume $0<p<1$. Let $G=G_n$ be a sequence of graphs on $n$ vertices with $p\binom n2(1+o(1))$ edges. 
        Assume further that all but $o(n)$ vertices have degree $pn(1+o(1))$. Then the following $6$ properties are 
        equivalent.
        \begin{itemize}
            \item \textbf{Property} $P^p_1$: For every graph $H(s,e)$ on $s$ vertices with $e$ edges
                $$
                N_G^*(H(s,e))=(1+o(1))n^sp^e(1-p)^{\binom s2-e}.
                $$
            \item \textbf{Property} $P^p_2$: For the cycle $C(4)$ with $4$ vertices, $N_G(C(4))\leq(1+o(1))p^4n^4$. 
            \item \textbf{Property} $P^p_3$: $\abs{\lambda_2}=o(n)$.
            \item \textbf{Property} $P^p_4$: For every set $S$ of vertices of $G$, $e(S)=\frac p2|S|^2+o(n^2)$.
            \item \textbf{Property} $P^p_5$: For every two sets of vertices $B,C$, $e(B,C)=p|B||C|+o(n^2)$.
            \item \textbf{Property} $P^p_6$: $\sum_{u,v\in V}\abs{|N(u)\cap N(v)|-p^2n}=o(n^3)$.
        \end{itemize}
    \end{theorem}
    \begin{proof}[$P_1^p\implies P^p_2$]
        Since $N_G(H)=\sum_{H\subseteq L}N_G^*(L)$, where $L$ is a graph on $|V(H)|$ vertices,
        we have
        \begin{align*}
            N_G(C(4))&=N_G^*(H(4,4))+2N_G^*(H(4,5))+N_G^*(H(4,6))\\
            &=(1+o(1))p^4n^4\sbra{(1-p)^2+2p(1-p)+p^2}\\
            &=(1+o(1))p^4n^4.
        \end{align*}
    \end{proof}
    \begin{proof}[$P_2^p\implies P^p_3$]
        Let $A$ be the adjacency matrix of $G$.
        By Perron-Frobenius Theorem, $\lambda_1>0$; thus
        $$
        \lambda_1=\sup_{x\in\Rbb^n}\frac{x^TAx}{x^Tx}\geq\frac{\bm 1^TA\bm 1}{\bm 1^T\bm 1}=pn(1+o(1)).
        $$
        On the other hand,
        $$
        (1+o(1))p^4n^4\geq N_G(C(4))=\tr\pbra{A^4}-o(n^4)=\sum_{i=1}^n\lambda_i^4-o(n^4)\geq p^4n^4(1+o(1))+\lambda_2^4-o(n^4),
        $$
        thus $|\lambda_2|=o(n)$.
    \end{proof}
    \begin{proof}[$P_3^p\implies P_4^p$]
        Let $A$ be the adjacency matrix of $G$.
        Let $\lambda_1,\cdots,\lambda_n$ be the eigenvalues of $G$ and $u_1,\cdots,u_n$ be the corresponding 
        orthonormal eigenvectors.
        \begin{lemma}
            $\vabs{u_1-\frac1{\sqrt n}\vec1}_2=o(1)$.
        \end{lemma}
        \begin{proof}
            Let $v_1=\frac1{\sqrt n}\vec1$ and $v_1=\sum_ia_iu_i$, then $pnv_1+e=Av_1=\sum_ia_i\lambda_iu_i$,
            where $\vabs{e}_2=o(n)$.
            Since by adding dummy edges we can get a $(pn(1+o(1)))$-regular graph, $\lambda_1=\vabs{A}_2\leq pn(1+o(1))$.
            Also, from the proof of $P_2^p\implies P_3^p$, we have $\lambda_1\geq pn(1+o(1))$; thus $\lambda_1=pn(1+o(1))$.
            Thus
            \begin{align*}
                &\sum_ia_i\lambda_iu_i=e+pnv_1=e+pn\pbra{\sum_ia_iu_i}\\
                \implies&\sum_{i>1}a_i\pbra{\lambda_i-pn}u_i=e+pn(pn-\lambda_1)u_1=e+o(n)u_1\\
                \implies&\vabs{\sum_{i>1}a_i\pbra{\lambda_i-pn}u_i}_2=\sqrt{\sum_{i>1}a_i^2(o(n)-pn)^2}=o(n)\\
                \implies&\sum_{i>1}a_i^2=o(1)\implies a_1=1-o(1)\\
                \implies&\vabs{u_1-\frac1{\sqrt n}\vec1}_2=\vabs{u_1-v_1}_2=(a_1-1)^2+\sum_{i>1}a_i^2=o(1).
            \end{align*}
        \end{proof}
        Without loss of generality, assume $|S|=\Theta(n)$, since otherwise $e(S)\leq|S|^2=o(n^2)$.
        Let $\vec1_S$ be the indicator vector of set $S$ and $\vec1_S=\sum_ib_iu_i$.
        Then
        $$
        b_1=\abra{\vec1_S,u_1}=\abra{\vec1_S,\frac1{\sqrt n}\vec1}+\abra{\vec1_S,u_1-\frac1{\sqrt n}\vec1}
        =\frac{|S|}{\sqrt n}+o(\sqrt{|S|})=\frac{|S|}{\sqrt n}+o(\sqrt{n}).
        $$
        Thus 
        $$
        2e(S)=\vec1_S^TA\vec1_S=\sum_i\lambda_ib_i^2=\pbra{\frac{|S|^2}{n}+o(n)}pn(1+o(1))+o(n)\pbra{\sum_{i>1}b_i^2}
        =p|S|^2+o(n^2).
        $$
    \end{proof}
    \begin{proof}[$P_4^p\implies P_5^p$]
        Let $D=B\cap C,B_1=B\backslash D,C_1=C\backslash D$. Then
        \begin{align*}
            e(B,C)&=e(B_1,D)+e(B_1,C_1)+e(D,C_1)+e(D)\\
            &=e(D)+\pbra{e(B_1\cup D)-e(B_1)-e(D)}
            +\pbra{e(B_1\cup C_1)-e(B_1)-e(C_1)}
            +\pbra{e(D\cup C_1)-e(D)-e(C_1)}\\
            &=\frac p2\pbra{\pbra{|B_1|+|D|}^2+\pbra{|B_1|+|C_1|}^2+\pbra{|D|+|C_1|}^2-2|B_1|^2-2|C_1|^2-|D|^2}+o(n^2)\\
            &=p\pbra{|B_1|+|D|}\pbra{|D|+|C_1|}+o(n^2)\\
            &=p|B||C|+o(n^2).
        \end{align*}
    \end{proof}
    \begin{proof}[$P_5^p\implies P_6^p$]
        Define $S=\cbra{u\in V\middle||N(u)|=pn(1+o(1))}$, then $|S|=n-o(n)$ and
        $$
        \sum_{u,v}\abs{|N(u)\cap N(v)|-p^2n}=
        \pbra{\sum_{u\in S}+\sum_{u\notin S}}\sum_v\abs{|N(u)\cap N(v)|-p^2n}
        =\sum_{u\in S}\sum_v\abs{|N(u)\cap N(v)|-p^2n}+o(n^3).
        $$
        Thus it suffices to show for any fixed $u\in S$
        $$
        \sum_v\abs{|N(u)\cap N(v)|-p^2n}=o(n^2).
        $$
        Let $T=\cbra{v\in V\middle||N(u)\cap N(v)|\geq p^2n}$, then
        \begin{align*}
            \sum_v\abs{|N(u)\cap N(v)|-p^2n}
            &=\pbra{\sum_{v\in T}N(u)\cap N(v)}-p^2n|T|
            -\pbra{\sum_{v\notin T}N(u)\cap N(v)}+p^2n(n-|T|)\\
            &=e(N(u),T)-e(N(u),T^c)+p^2n(n-2|T|)\\
            &=p|N(u)|(|T|-n+|T|)+o(n^2)+p^2n(n-2|T|)\\
            &=p^2n(1+o(1))(2|T|-n)+o(n^2)+p^2n(n-2|T|)\\
            &=o(n^2).
        \end{align*}
    \end{proof}
    \begin{proof}[$P_6^p\implies P_1^p$]
        Prove by induction on $s$. 
        
        If $s=1$, then $e=0$ and $N_G^*(H(s,e))=n$. 

        Now we assume $s=k+1,k\geq1$.
        Let $V(H(k+1,e))=v_1,\cdots,v_{k+1}$ and $H'$ be the graph induced by $v_1,\cdots,v_k$.
        Denote $A$ as the adjacency matrix of G and
        $$
        s_b(u,v)=\#\cbra{w\in G\backslash\cbra{u,v}\middle|A_{u,w}=A_{v,w}=b}
        $$
        for $b\in\bin$.
        Let $I_i=1$ if $v_{k+1}$ is linked with $v_i$ and $I_i=0$ otherwise.
        Denote $\Delta=|I|=\sum_iI_i$ and 
        $f$ as 
        $$
        f(w_1,\cdots,w_k)=\#\cbra{x\in G\backslash\cbra{w_1,\cdots,w_k}\middle|A_{x,w_i}=I_i}.
        $$
        Then $N_G^*(H(k+1,e))$ is the summation of $f(w)$ if $G\restriction_w=H'$

        Consider the uniform distribution over $w\in G_{(k)}$. Then
        \begin{align*}
            \mu
            &=\E_w\sbra{f(w)}=\frac1{n_{(k)}}\sum_{w_1,\cdots,w_k}f(w_1,\cdots,w_k)\\
            &=\frac1{n_{(k)}}\sum_{x\in V}\sum_{w_1,\cdots,w_k}[w_1,\cdots,w_k,x\text{ is valid}]\\
            &=\frac1{n_{(k)}}\sum_{x\in V}d(x)_{(\Delta)}\pbra{n-1-d(x)}_{(k-\Delta)}\\
            &=\frac1{n_{(k)}}\pbra{n(pn)_{(\Delta)}(n-1-pn)_{(k-\Delta)}+o(n)n_{(k)}}\\
            &=p^\Delta(1-p)^{k-\Delta}n+o(n)
        \end{align*}
        and 
        \begin{align*}
            \E_w\sbra{f^2(w)}
            &=\frac1{n_{(k)}}\sum_wf^2(w)\\
            &=\frac1{n_{(k)}}\sum_{x,y\in V}\sum_{w_1,\cdots,w_k}[w_1,\cdots,w_k,x\text{ and }w_1,\cdots,w_k,y\text{ are valid}]\\
            &=\frac1{n_{(k)}}\sum_{x,y\in V}s_1(x,y)_{(\Delta)}s_0(x,y)_{(k-\Delta)}\\
            &=\frac1{n_{(k)}}\sum_{x,y\in V}|N(x)\cap N(y)|_{(\Delta)}\pbra{n-2-|N(x)|-|N(y)|+|N(x)\cap N(y)|}_{(k-\Delta)}\\
            &=o(n^2)+\frac1{n_{(k)}}\sum_{x,y\in V}|N(x)\cap N(y)|_{(\Delta)}\pbra{(1-2p)n+|N(x)\cap N(y)|}_{(k-\Delta)}.
        \end{align*}

        Let $\epsilon_{x,y}=|N(x)\cap N(y)|-p^2n$, then $\abs{\epsilon_{x,y}}\leq n$ and by 
        \textbf{Property $P_6^p$}, we have $\sum_{x,y\in V}\abs{\epsilon_{x,y}}=o(n^3)$.
        Thus
        \begin{align*}
            \E_w\sbra{f^2(w)}
            &=o(n^2)+\frac1{n_{(k)}}\sum_{x,y\in V}\pbra{p^2n+\epsilon_{x,y}}_{(\Delta)}
            \pbra{(1-p)^2n+\epsilon_{x,y}}_{(k-\Delta)}\\
            &=o(n^2)+\frac1{n_{(k)}}\sum_{x,y\in V}\sum_{d=0}^k\epsilon_{x,y}^d
            \sum_{i=0}^dc_{x,y,d,i}\pbra{p^2n}^{\Delta-i}\pbra{(1-p)^2n}^{k-\Delta-d+i}\\
            &=o(n^2)+\frac1{n_{(k)}}\sum_{x,y\in V}\pbra{
                \pbra{p^\Delta(1-p)^{k-\Delta}}^2n^k+
                \sum_{d=1}^k\epsilon_{x,y}^d
            \sum_{i=0}^dc_{x,y,d,i}\pbra{p^2n}^{\Delta-i}\pbra{(1-p)^2n}^{k-\Delta-d+i}}\\
            &=o(n^2)+\frac1{n_{(k)}}\pbra{p^\Delta(1-p)^{k-\Delta}}^2n^{k+2}
                +\sum_{d=1}^kO(n^{k-d})\sum_{x,y\in V}\epsilon_{x,y}^d\\
            &\leq o(n^2)+\frac1{n_{(k)}}\pbra{p^\Delta(1-p)^{k-\Delta}}^2n^{k+2}
                +\sum_{d=1}^kO(n^{k-d})O(n^{d-1})\pbra{\sum_{x,y\in V}\abs{\epsilon_{x,y}}}\\
            &\leq o(n^2)+\frac1{n_{(k)}}\pbra{p^\Delta(1-p)^{k-\Delta}}^2n^{k+2}
                +\frac1{n_{(k)}}\sum_{d=1}^kO(n^{k-d})O(n^{d-1})o(n^3)\\
            &=\pbra{p^\Delta(1-p)^{k-\Delta}}^2n^2+o(n^2).
        \end{align*}
        Therefore
        \begin{align*}
            \abs{N_G^*(H(k+1,e))-N_G^*(H')\mu}
            &=\abs{\sum_{w,G\restriction_w=H'}f(w)-\mu}\\
            &\leq\sqrt{N_G^*(H')\sum_{w,G\restriction_w=H'}(f(w)-\mu)^2}\\
            &\leq\sqrt{N_G^*(H')\sum_w(f(w)-\mu)^2}\\
            &\leq\sqrt{N_G^*(H')n_{(k)}\pbra{\E\sbra{f^2(w)}-\mu^2}}\\
            &\leq\sqrt{(1+o(1))n^kp^{e(H')}(1-p)^{\binom k2-e(H')}n_{(k)}o(n^2)}\\
            &=o(n^{k+1}),
        \end{align*}
        which gives
        \begin{align*}
        N_G^*(H(k+1,e))
            &=N_G^*(H')\mu+o(n^{k+1})=n^kp^{e(H')}(1-p)^{\binom k2-e(H')}p^\Delta(1-p)^{k-\Delta}n+o(n^{k+1})\\
            &=(1+o(1))n^{k+1}p^e(1-p)^{\binom{k+1}2-e}
        \end{align*}
        as desired.
    \end{proof}
\end{exercise}

\end{document}
