% !TeX encoding = UTF-8
% !TeX program = XeLaTeX
% !TeX spellcheck = LaTeX

\documentclass[a4paper]{article}

\usepackage[UTF8]{ctex}
\usepackage{amsmath,amsfonts,amssymb}
\usepackage{mathrsfs}
\usepackage{bm}
\usepackage{extarrows}
\usepackage{geometry}
\usepackage{ntheorem}
\usepackage{hyperref}
\usepackage[ruled]{algorithm2e}
\usepackage{caption,subcaption}

\geometry{left=2cm,right=2cm,top=2cm,bottom=2cm}

\def\UrlBreaks{\do\A\do\B\do\C\do\D\do\E\do\F\do\G\do\H\do\I\do\J\do\K\do\L\do\M\do\N\do\O\do\P\do\Q\do\R\do\S\do\T\do\U\do\V\do\W\do\X\do\Y\do\Z\do\[\do\\\do\]\do\^\do\_\do\`\do\a\do\b\do\c\do\d\do\e\do\f\do\g\do\h\do\i\do\j\do\k\do\l\do\m\do\n\do\o\do\p\do\q\do\r\do\s\do\t\do\u\do\v\do\w\do\x\do\y\do\z\do\0\do\1\do\2\do\3\do\4\do\5\do\6\do\7\do\8\do\9\do\.\do\@\do\\\do\/\do\!\do\_\do\|\do\;\do\>\do\]\do\)\do\,\do\?\do\'\do+\do\=\do\#}

\newtheorem{theorem}{Theorem}
\newtheorem{lemma}{Lemma}
\newtheorem{proposition}{Proposition}
\newtheorem{corollary}{Corollary}
\newtheorem{claim}{Claim}
\newtheorem{conjecture}{conjecture}
\newtheorem{definition}{Definition}
\newtheorem{construction}{Construction}
\newtheorem*{proof}{Proof}
\newtheorem*{answer}{Answer}
\newtheorem*{refute}{Refute}
\newtheorem*{example}{Example}
\newtheorem*{counterexample}{Counterexample}

\newenvironment{exercise}[1]{
	\par
	\noindent\textbf{Exercise #1.}\quad
}{
	\par
	\bigskip
}


\DeclareMathAccent{\widehat}{\mathord}{largesymbols}{"62}
\newcommand{\abs}[1]{\left| #1 \right|}
\newcommand{\pbra}[1]{\left( #1 \right)}
\newcommand{\cbra}[1]{\left\{ #1 \right\}}
\newcommand{\sbra}[1]{\left[ #1 \right]}
\newcommand{\bin}{\{0,1\}}

\title{Exercise Set --- Chapter $2$}
\date{}

\begin{document}

\maketitle

\begin{exercise}{2}
    It's easy to see $x([x>0]-[x<0])=|x|$.
\end{exercise}

\begin{exercise}{7}
    $$
    \nabla\pbra{x^{\overline m}}=x^{\overline m}-(x-1)^{\overline m}
    =x(x+1)\cdots(x+m-1)-(x-1)x\cdots(x+m-2)=mx^{\overline{m-1}}.
    $$
\end{exercise}

\begin{exercise}{12}
    Assume $p(k)=p(\ell)$, we have $k-\ell=c\pbra{(-1)^\ell-(-1)^k}$.
    \begin{itemize}
        \item $k=2u,\ell=2v$: $2(u-v)=0\implies u=v\implies k=\ell$.
        \item $k=2u+1,\ell=2v$: $2(u-v)+1=-2c$, impossible.
        \item $k=2u,\ell=2v+1$: $2(u-v)-1=2c$, impossible.
        \item $k=2u+1,\ell=2v+1$: $2(u-v)=0\implies u=v\implies k=\ell$.
    \end{itemize}
\end{exercise}

\end{document}
