
% !TeX encoding = UTF-8
% !TeX program = XeLaTeX
% !TeX spellcheck = LaTeX

\documentclass[a4paper]{article}

\usepackage{amsthm,amsmath,amsfonts,amssymb}
\usepackage{mathrsfs}
\usepackage{bm}
\usepackage{geometry}
% \usepackage{ntheorem}
\usepackage{hyperref}
\usepackage[ruled]{algorithm2e}
\usepackage{caption,subcaption}

\geometry{left=2cm,right=2cm,top=2cm,bottom=2cm}

\def\UrlBreaks{\do\A\do\B\do\C\do\D\do\E\do\F\do\G\do\H\do\I\do\J\do\K\do\L\do\M\do\N\do\O\do\P\do\Q\do\R\do\S\do\T\do\U\do\V\do\W\do\X\do\Y\do\Z\do\[\do\\\do\]\do\^\do\_\do\`\do\a\do\b\do\c\do\d\do\e\do\f\do\g\do\h\do\i\do\j\do\k\do\l\do\m\do\n\do\o\do\p\do\q\do\r\do\s\do\t\do\u\do\v\do\w\do\x\do\y\do\z\do\0\do\1\do\2\do\3\do\4\do\5\do\6\do\7\do\8\do\9\do\.\do\@\do\\\do\/\do\!\do\_\do\|\do\;\do\>\do\]\do\)\do\,\do\?\do\'\do+\do\=\do\#}

\newtheorem{theorem}{Theorem}
\newtheorem{lemma}{Lemma}
\newtheorem{proposition}{Proposition}
\newtheorem{corollary}{Corollary}
\newtheorem{claim}{Claim}
\newtheorem{conjecture}{conjecture}
\newtheorem{definition}{Definition}
\newtheorem{construction}{Construction}
\newtheorem*{answer}{Answer}
\newtheorem*{refute}{Refute}
\newtheorem*{example}{Example}
\newtheorem*{counterexample}{Counterexample}

\newenvironment{exercise}[1]{
	\par
	\noindent\textbf{Exercise #1.}\quad
}{
	\par
	\bigskip
}


\DeclareMathAccent{\widehat}{\mathord}{largesymbols}{"62}
\newcommand{\abs}[1]{\left| #1 \right|}
\newcommand{\vabs}[1]{\left\| #1 \right\|}
\newcommand{\pbra}[1]{\left( #1 \right)}
\newcommand{\cbra}[1]{\left\{ #1 \right\}}
\newcommand{\sbra}[1]{\left[ #1 \right]}
\newcommand{\bin}{\{0,1\}}


\def\sD{\textsf{D}}
\def\sE{\textsf{E}}
\def\cD{\mathcal{D}}

\title{Exercise Set --- Chapter 21}
\date{}

\begin{document}
    \maketitle

    \begin{exercise}{21.9}
        By reordering vertices in $G$, we assume 
        $$
        \bm A=\begin{bmatrix}
            &\bm B\\
            \bm C & 
        \end{bmatrix},
        $$
        where $\bm B$ is $a$ by $n-a$ and $\bm C$ is $n-a$ by $a$.
        Since 
        $$
        \bm A\begin{bmatrix}1\\\vdots\\1\end{bmatrix}=\begin{bmatrix}1\\\vdots\\1\end{bmatrix},
        $$
        we have
        $$
        \bm A\begin{bmatrix}-1\\\vdots\\-1\\1\\\vdots\\1\end{bmatrix}
        =\begin{bmatrix}&\bm B\\\bm C &\end{bmatrix}\begin{bmatrix}-1\\\vdots\\-1\\1\\\vdots\\1\end{bmatrix}
        =\begin{bmatrix}1\\\vdots\\1\\-1\\\vdots\\-1\end{bmatrix}.
        $$
    \end{exercise}

    \begin{exercise}{21.14}
        Let $\bm A$ be the random walk matrix of $G$ and
        $$
        (\bm 1_S)_i=\begin{cases}
            \frac1{|S|} & i\in S\\
            0 & i\notin S
        \end{cases},\quad
        (\bm 1_T)_i=\begin{cases}
            \frac1{|T|} & i\in S\\
            0 & i\notin S
        \end{cases},\quad
        \bm e=\frac1{\sqrt n}\begin{bmatrix}1\\\vdots\\1\end{bmatrix}.
        $$
        Then $\bm 1_T=\frac1{\sqrt n}\bm e+\alpha$, where $\alpha$ is orthogonal to $\bm e$, and 
        \begin{align*}
            \abs{\frac{|E(S,T)|}{d|S||T|}-\frac1n}
            &=\abs{\bm 1_S^\top\bm A\bm 1_T-\frac1n}
            =\abs{\bm 1_S^\top\bm A\pbra{\frac1{\sqrt n}\bm e+\alpha}-\frac1n}
            =\abs{\bm 1_S^\top\bm A\alpha}
            =\vabs{\bm 1_S^\top\bm A\alpha}_2\\
            &\leq\vabs{\bm1_S}_2\vabs{\bm A\alpha}_2
            \leq\frac\lambda{\sqrt{|S|}}\vabs{\alpha}_2
            <\frac\lambda{\sqrt{|S|}}\vabs{\bm1_T}_2\\
            &=\frac\lambda{\sqrt{|S||T|}}.
        \end{align*}
    \end{exercise}

\end{document}
